theories/Theorems/Order.v
@@ -1,5 +1,9 @@
 Require Import Utf8.Spec.
 From Coq Require Import Lists.List. Import ListNotations.
+From Coq Require Import NArith.BinNat.
+From Coq Require Import Hexadecimal.
+From Coq Require Import Strings.Byte.
+From Coq Require Import Lia.
 
 Ltac crush_bits :=
   let B := fresh "B" in
@@ -35,6 +39,125 @@ Ltac to_bits byte :=
       rewrite Byte.of_bits_to_bits in eqn_name
   end.
 
+Definition c0800 := N.of_hex_uint (D8 (D0 (D0 Nil))).
+Definition ce000 := N.of_hex_uint (De (D0 (D0 (D0 Nil)))).
+
+Definition nth_valid_codepoint (n: N) : option codepoint :=
+  if (n <? cd800)%N then
+    Some n
+  else if (n <=? c10ffff - c0800)%N then
+    Some (n + c0800)%N
+  else
+    None.
+
+Lemma nth_valid_codepoint_is_some_implies_valid : forall n code,
+    nth_valid_codepoint n = Some code ->
+    valid_codepoint code.
+Proof.
+  intros n code nth.
+  unfold valid_codepoint, codepoint_less_than_10ffff, codepoint_is_not_surrogate.
+  unfold nth_valid_codepoint in nth.
+  destruct (n <? cd800)%N eqn:less_than_d800; inversion nth; subst; clear nth.
+  - apply N.ltb_lt in less_than_d800.
+    split. apply N.lt_le_incl in less_than_d800. apply N.le_trans with (m:= cd800). assumption. vm_compute. easy.
+    left. assumption.
+  - apply N.ltb_nlt in less_than_d800.
+    destruct (n <=? 1112063)%N eqn:less_than_10ffff_m_800; [| discriminate].
+    apply N.leb_le in less_than_10ffff_m_800.
+    inversion H0. subst. clear H0.
+    split. replace (1112063)%N with (c10ffff - c0800)%N in less_than_10ffff_m_800 by reflexivity.
+    specialize (N.add_le_mono_r n (c10ffff - c0800)%N c0800) as [G1 G2].
+    apply G1 in less_than_10ffff_m_800.
+    rewrite N.sub_add in less_than_10ffff_m_800.
+    apply less_than_10ffff_m_800. vm_compute. intro. discriminate.
+    apply N.nlt_ge in less_than_d800.
+    right. apply N.lt_gt.
+    specialize (N.add_le_mono_r cd800 n c0800) as [G1 G2].
+    apply G1 in less_than_d800.
+    replace (cd800 + c0800)%N with (ce000) in less_than_d800 by reflexivity.
+    specialize (N.lt_succ_diag_r cdfff) as s. replace (N.succ cdfff) with ce000 in s by reflexivity.
+    lia.
+Qed.
+    
+Definition inverse_nth_valid_codepoint (code: codepoint) : option N :=
+  if (code <? cd800)%N then
+    Some code
+  else if (code <=? c10ffff)%N then
+    Some (code - c0800)%N
+  else
+    None.
+
+Theorem nth_valid_codepoint_invertible : forall code n,
+    nth_valid_codepoint n = Some code <->
+      inverse_nth_valid_codepoint code = Some n /\ valid_codepoint code.
+Proof.
+  intros code n.
+  split; intros.
+  - apply nth_valid_codepoint_is_some_implies_valid in H as code_valid. split; [|apply code_valid].
+    unfold inverse_nth_valid_codepoint. unfold nth_valid_codepoint in H.
+    destruct (n <? cd800)%N eqn:less_than_d800.
+    + inversion H. subst. rewrite less_than_d800. reflexivity.
+    + apply N.ltb_nlt in less_than_d800.
+      destruct (n <=? c10ffff - c0800)%N eqn:less_than_10ffff; [| discriminate].
+      inversion H. subst. clear H.
+      apply N.leb_le in less_than_10ffff.
+      destruct (n + cdfff <? cd800)%N eqn:plus_less_than_d800.
+      apply N.ltb_lt in plus_less_than_d800. lia.
+      apply N.ltb_nlt in plus_less_than_d800.
+      destruct (n + c0800 <? cd800)%N eqn:plus_less_than_cd800.
+      * apply N.ltb_lt in plus_less_than_cd800. lia.
+      * apply N.ltb_nlt in plus_less_than_cd800.
+        destruct (n + c0800 <=? c10ffff)%N eqn: plus_less_than_10ffff.
+        -- rewrite N.add_sub. reflexivity.
+        -- apply N.leb_nle in plus_less_than_10ffff.
+           apply N.add_le_mono_r with (p:=c0800) in less_than_10ffff. 
+           rewrite N.sub_add in less_than_10ffff. 
+           lia. unfold N.le. intro G. simpl in G. vm_compute in G. discriminate.
+  - destruct H as [H valid_code].
+    unfold inverse_nth_valid_codepoint in H.
+    unfold valid_codepoint, codepoint_less_than_10ffff, codepoint_is_not_surrogate in valid_code.
+    destruct valid_code as [code_less_than_10ffff code_not_surrogate].
+    unfold nth_valid_codepoint.
+    destruct (N.ltb code cd800) eqn:less_than_d800.
+    + inversion H. subst. rewrite less_than_d800. reflexivity.
+    + apply N.ltb_nlt in less_than_d800.
+      destruct (code <=? c10ffff)%N eqn:less_than_10ffff; [| discriminate].
+      inversion H. subst. clear H.
+      apply N.leb_le in less_than_10ffff.
+      destruct (code - c0800 <? cd800)%N eqn: plus_less_than_cdfff.
+      * apply N.ltb_lt in plus_less_than_cdfff.
+        apply N.nlt_ge in less_than_d800. destruct code_not_surrogate; try lia.
+        apply N.add_lt_mono_r with (p:=c0800) in plus_less_than_cdfff.
+        rewrite N.sub_add in plus_less_than_cdfff.
+        apply N.gt_lt in H.
+        apply N.succ_lt_mono in H. 
+        replace (cd800 + c0800)%N with ce000 in plus_less_than_cdfff by reflexivity.
+        replace (N.succ cdfff) with ce000 in H by reflexivity. lia.
+        apply (N.le_trans) with (m := cd800). vm_compute. intro G. discriminate G. assumption.
+      * apply N.ltb_nlt in plus_less_than_cdfff.
+        destruct (code - c0800 <=? c10ffff - c0800)%N eqn:plus_less_than_10ffff_m_800.
+        -- rewrite N.sub_add. reflexivity.
+           apply N.nlt_ge in less_than_d800.
+           apply N.le_trans with (m:= cd800).  vm_compute. intro G. discriminate G. assumption.
+        -- apply N.leb_nle in plus_less_than_10ffff_m_800.
+           lia.
+Qed.
+        
+Definition nth_valid_codepoint_representation (n: N) : option (list byte).
+  destruct (Nat.leb n 127) eqn:E.
+  assert (n < 255) as valid_byte. 
+  apply PeanoNat.Nat.leb_le in E. lia.
+  destruct (of_nat n) eqn:b.
+  2: { apply of_nat_None_iff in b. lia. } 
+  apply (Some [b0]).
+  apply None.
+Defined.
+
+From Coq Require Extraction.
+Extraction nth_valid_byte.
+      
+  
+
 Lemma byte_compare_antisymmetric : forall byte1 byte2, byte_compare byte1 byte2 = CompOpp (byte_compare byte2 byte1).
 Proof.
   intros byte1 byte2.
@@ -61,3 +184,4 @@ Proof.
   apply list_compare_refl; [| reflexivity].
   apply cmp_eq.
 Qed.
+
