theories/Theorems/Spec.v
@@ -7,99 +7,60 @@ Require Import Utf8.Parser.
 Require Import Utf8.Spec.
 Require Import Utf8.Theorems.Order.
 
-Ltac destruct_valid_bytes valid_bytes :=
-  let start R :=
-    match type of R with
-    | valid_utf8_bytes (cons ?head ?tail) => idtac
-    | valid_utf8_bytes ?bytes =>
-        let head := fresh "byte" in
-        let tail := fresh "byte_rest" in
-        let bytes := fresh "bytes_eq" in
-        destruct bytes as [|head tail] eqn:bytes
-    end;
-    unfold valid_utf8_bytes in valid_bytes;
-    fold valid_utf8_bytes in valid_bytes;
-    match type of R with
-    | context[byte_range ?byte] =>
-        let byte_in_range := fresh "byte_in_range" in
-        destruct (byte_range byte) eqn:byte_in_range; try contradiction
-    end
-  in
-let rec go R :=
-  unfold expect in R;
-  match type of R with
-  | valid_utf8_bytes ?b => idtac
-  | match ?bytes with | _ => _ end =>
-      let head := fresh "byte" in
-      let tail := fresh "byte_rest" in
-      let bytes_eq := fresh "bytes_eq" in
-      let byte_pred := fresh "byte_pred" in 
-      let rest_pred := fresh "rest_pred" in
-      destruct bytes as [| head tail] eqn:bytes_eq; try contradiction;
-      destruct R as [byte_pred rest_pred];
-      go rest_pred
-  end in
-  start valid_bytes; go valid_bytes.
-
-Theorem valid_utf8_bytes_concat_strong : forall (bytes_big bytes1 bytes2: list byte),
-    (length bytes1) <= (length bytes_big) ->
-    valid_utf8_bytes bytes1 ->
-    valid_utf8_bytes bytes2 ->
-    valid_utf8_bytes (bytes1 ++ bytes2).
-Proof.
-  intros bytes_big. induction bytes_big; intros bytes1 bytes2 lesser bytes1_valid bytes2_valid.
-  inversion lesser. apply List.length_zero_iff_nil in H0. subst. apply bytes2_valid.
-  destruct bytes1 as [| byte1 rest1]; auto.
-  simpl in bytes1_valid |- *.
-  destruct (byte_range byte1); auto;
-  let rec prove_concat :=
-    match goal with
-    | |- valid_utf8_bytes (?b1 ++ ?b2) =>
-        apply IHbytes_big; simpl in lesser; try lia; assumption
-    | [G: expect ?byte_pred1 ?rest_pred1 ?b1 |- expect ?byte_pred2 ?rest_pred2 (?b1 ++ ?b2)] =>
-        let byte := fresh "byte_in_range" in
-        let rest := fresh "rest_pred" in
-        simpl in G |- *; destruct b1; simpl in G |- *; try easy;
-        destruct G as [byte rest];
-        split; try apply byte; prove_concat
-  end
-  in prove_concat.
-Qed.
+(* Ltac destruct_valid_bytes valid_bytes := *)
+(*   let start R := *)
+(*     match type of R with *)
+(*     | valid_utf8_bytes (cons ?head ?tail) => idtac *)
+(*     | valid_utf8_bytes ?bytes => *)
+(*         let head := fresh "byte" in *)
+(*         let tail := fresh "byte_rest" in *)
+(*         let bytes_eq := fresh "bytes_eq" in *)
+(*         destruct bytes as [|head tail] eqn:bytes_eq *)
+(*     end; *)
+(*     unfold valid_utf8_bytes in valid_bytes; *)
+(*     fold valid_utf8_bytes in valid_bytes; *)
+(*     match type of R with *)
+(*     | context[byte_range ?byte] => *)
+(*         let byte_in_range := fresh "byte_in_range" in *)
+(*         destruct (byte_range byte) eqn:byte_in_range; try contradiction *)
+(*     end *)
+(*   in *)
+(* let rec go R := *)
+(*   unfold expect in R; *)
+(*   match type of R with *)
+(*   | valid_utf8_bytes ?b => idtac *)
+(*   | match ?bytes with | _ => _ end => *)
+(*       let head := fresh "byte" in *)
+(*       let tail := fresh "byte_rest" in *)
+(*       let bytes_eq := fresh "bytes_eq" in *)
+(*       let byte_pred := fresh "byte_pred" in  *)
+(*       let rest_pred := fresh "rest_pred" in *)
+(*       destruct bytes as [| head tail] eqn:bytes_eq; try contradiction; *)
+(*       destruct R as [byte_pred rest_pred]; *)
+(*       go rest_pred *)
+(*   end in *)
+(*   start valid_bytes; go valid_bytes. *)
 
 Theorem valid_utf8_bytes_concat : forall (bytes1 bytes2: list byte),
     valid_utf8_bytes bytes1 ->
     valid_utf8_bytes bytes2 ->
     valid_utf8_bytes (bytes1 ++ bytes2).
 Proof.
-  intros bytes1 bytes2 valid_bytes1 valid_bytes2.
-  apply valid_utf8_bytes_concat_strong with (bytes_big := bytes1). lia.
-  1,2: assumption.
+  intros bytes1 bytes2 valid_bytes1. induction valid_bytes1; intros valid_bytes2. assumption.
+  rewrite <- app_assoc. apply Utf8Concat. apply H. apply IHvalid_bytes1. apply valid_bytes2.
 Qed.
 
-Theorem valid_utf8_decompose_strong : forall (bytes_big bytes1 bytes2: list byte),
-    (length bytes1) <= (length bytes_big) -> 
+Theorem valid_utf8_decompose : forall (bytes1 bytes2: list byte),
     valid_utf8_bytes (bytes1 ++ bytes2) ->
     valid_utf8_bytes bytes1 ->
     valid_utf8_bytes bytes2.
 Proof.
-  intros bytes_big.
-  induction bytes_big.
-  - intros. inversion H. rewrite List.length_zero_iff_nil in H3. subst. simpl in H0. apply H0.
-  - intros bytes1 bytes2 LessThan bytes_concat_valid bytes1_valid.
-    destruct bytes1.
-    + apply bytes_concat_valid.
-    + rewrite <- List.app_comm_cons in bytes_concat_valid.
-      destruct_valid_bytes bytes1_valid; destruct_valid_bytes bytes_concat_valid; try discriminate;
-      repeat match goal with
-             | [G: ((?byte1 :: ?bs1) ++ ?bs2)%list = (?byte2 :: ?bs3)%list |- _] =>
-                 inversion G; subst
-             | _ => idtac
-             end; 
-        match goal with 
-        | [G1: valid_utf8_bytes ?bytes1, G2: valid_utf8_bytes (?bytes1 ++ ?bytes2) |- valid_utf8_bytes ?bytes2] => 
-            apply (IHbytes_big bytes1 bytes2); try (simpl in *; lia); repeat assumption
-        end.
-Qed.
+  intros bytes1 bytes2 valid_concat valid_bytes1. induction valid_bytes1.
+  - assumption.
+  - rewrite <- app_assoc in valid_concat.
+    inversion valid_concat. symmetry in H1. apply app_eq_nil in H1. destruct H1. apply app_eq_nil in H1. destruct H1. subst. constructor.
+    Admitted.
+
 
 Lemma list_equals_self_append_implies_nil {T}: forall (list1 list2: list T),
     list1 = list1 ++ list2 ->
@@ -149,6 +110,166 @@ Proof.
   unfold codepoints_compare in compare_codes. apply list_compare_refl in compare_codes. apply compare_codes.
   apply Z.compare_eq_iff.
 Qed.
+
+Lemma decoder_spec_injective : forall decoder,
+    utf8_decoder_spec decoder ->
+    forall (bytes1 bytes2: list byte) codes,
+      decoder bytes1 = (codes, []) ->
+      decoder bytes2 = (codes, []) ->
+      bytes1 = bytes2.
+Proof.
+  intros decoder decoder_spec_compliant.
+  assert (G := decoder_spec_compliant).
+  unfold utf8_decoder_spec, decoder_decode_correctly_implies_valid, decoder_decode_valid_utf8_bytes_correctly, decoder_strictly_increasing in G.
+  destruct G as [dec_implies_valid_utf8_bytes [valid_bytes_iff_enc dec_strictly_increasing]].
+  intros bytes1 bytes2 codes decoder_bytes1 decoder_bytes2.
+  specialize (dec_strictly_increasing bytes1 bytes2 codes codes decoder_bytes1 decoder_bytes2) as compare_codes.
+  unfold codepoints_compare in compare_codes.
+  rewrite list_compare_refl_if in compare_codes. 2: apply Z.compare_eq_iff.
+  unfold bytes_compare in compare_codes. symmetry in compare_codes. rewrite list_compare_refl in compare_codes.
+  apply compare_codes. apply byte_compare_eq_iff.
+Qed.
+
+Lemma decoder_spec_projects_inverse: forall decoder,
+    utf8_decoder_spec decoder ->
+    forall bytes codes1 codes2,
+      decoder bytes = (codes1 ++ codes2, []) ->
+      exists bytes1 bytes2,
+        decoder bytes1 = (codes1, []) /\
+          decoder bytes2 = (codes2, []) /\
+          bytes = bytes1 ++ bytes2.
+Admitted.
+
+Lemma decoder_spec_decode_app_valid_bytes : forall decoder,
+    utf8_decoder_spec decoder ->
+    forall bytes1 bytes2,
+      valid_utf8_bytes bytes1 ->
+      valid_utf8_bytes bytes2 ->
+      decoder (bytes1 ++ bytes2) =
+        let '(codes1, rest1) := decoder bytes1 in
+        let '(codes2, rest2) := decoder bytes2 in
+        (codes1 ++ codes2, []).
+Proof.
+  intros decoder decoder_spec_compliant.
+  assert (G := decoder_spec_compliant).
+  unfold utf8_decoder_spec, decoder_decode_correctly_implies_valid, decoder_decode_valid_utf8_bytes_correctly, decoder_strictly_increasing in G.
+  destruct G as [dec_implies_valid_utf8_bytes [valid_bytes_iff_enc dec_strictly_increasing]].
+  Admitted.
+
+Lemma decoder_spec_nil_mapsto_nil : forall decoder,
+    utf8_decoder_spec decoder ->
+    decoder nil = (nil, []).
+  intros decoder decoder_spec_compliant.
+  assert (G := decoder_spec_compliant).
+  unfold utf8_decoder_spec, decoder_decode_correctly_implies_valid, decoder_decode_valid_utf8_bytes_correctly, decoder_strictly_increasing in G.
+  destruct G as [dec_implies_valid_utf8_bytes [valid_bytes_iff_dec dec_strictly_increasing]].
+  assert (valid_utf8_bytes []) as nil_valid. constructor. apply valid_bytes_iff_dec in nil_valid as G.
+  destruct G as [codes decode_codes].
+  assert (decode_codes_copy := decode_codes).
+  replace (nil) with (@nil byte ++ @nil byte) in decode_codes by reflexivity.
+  rewrite decoder_spec_decode_app_valid_bytes in decode_codes; try assumption.
+  rewrite decode_codes_copy in decode_codes.
+  inversion decode_codes. symmetry in H0.
+  apply list_equals_self_append_implies_nil in H0.
+  subst. assumption.
+Qed.
+
+Lemma encoder_spec_implies_nth_code_mapsto_nth_byte : forall encoder,
+    utf8_encoder_spec encoder ->
+    forall code bytes,
+      encoder [code] = (bytes, []) -> 
+      exists n, nth_valid_codepoint n = Some code /\ nth_valid_byte n = Some bytes.
+Admitted.
+
+Lemma decoder_spec_implies_nth_bytes_mapsto_nth_code : forall decoder,
+    utf8_decoder_spec decoder ->
+    forall bytes code,
+      decoder bytes = ([code], []) -> 
+      exists n, nth_valid_codepoint n = Some code /\ nth_valid_byte n = Some bytes.
+Admitted.
+
+Theorem decode_encode_spec_inverses_for_single: forall encoder decoder,
+    utf8_encoder_spec encoder ->
+    utf8_decoder_spec decoder ->
+    forall code bytes,
+      encoder [code] = (bytes, []) ->
+      decoder bytes = ([code], []).
+Proof.
+  intros encoder decoder encoder_spec_compliant decoder_spec_compliant.
+  assert (G1 := encoder_spec_compliant).
+  assert (G2 := decoder_spec_compliant).
+  destruct G1 as [enc_implies_valid_utf8_bytes [valid_codepoints_iff_enc [enc_strictly_increasing enc_projects]]].
+  destruct G2 as [dec_implies_valid [valid_implies_dec dec_strictly_increasing]].
+  intros code bytes encode_code.
+  apply enc_implies_valid_utf8_bytes in encode_code as G. destruct G as [bytes_valid _].
+  apply valid_implies_dec in bytes_valid as G. destruct G as [codes decode_bytes].
+  apply dec_implies_valid in decode_bytes as G. destruct G as [codes_valid _].
+  apply valid_codepoints_iff_enc in codes_valid as G. destruct G as [bytes2 encode_codes].
+  specialize (enc_strictly_increasing [code] codes bytes bytes2 encode_code encode_codes) as compare_code_codes.
+  specialize (encoder_spec_implies_nil_mapsto_nil encoder encoder_spec_compliant) as encode_nil.
+  specialize (decoder_spec_nil_mapsto_nil decoder decoder_spec_compliant) as decode_nil.
+  destruct codes as [|code2 codes_rest].
+  - specialize (decoder_spec_injective decoder decoder_spec_compliant [] bytes [] decode_nil decode_bytes) as G.
+    subst. simpl in compare_code_codes. destruct bytes2; discriminate.
+  - replace (code2 :: codes_rest) with ([code2] ++ codes_rest) in encode_codes, decode_bytes, codes_valid, compare_code_codes by reflexivity.
+    rewrite enc_projects in encode_codes.
+    destruct (encoder [code2]) as [bytes3 rest] eqn:encode_code2.
+    destruct (encoder codes_rest) as [bytes4 rest2] eqn:encode_codes_rest.
+    destruct rest; [|discriminate]. inversion encode_codes. subst. clear encode_codes.
+    specialize (enc_strictly_increasing [code] [code2] bytes bytes3 encode_code encode_code2) as compare_code_code2.
+    apply decoder_spec_projects_inverse in decode_bytes. 2: assumption.
+    destruct decode_bytes as [bytes1 [bytes2 [decode_bytes1 [decode_bytes2 bytes_eq]]]].
+    rewrite bytes_eq in compare_code_codes, compare_code_code2, encode_code, bytes_valid |- *.
+    destruct bytes1. rewrite decode_nil in decode_bytes1. inversion decode_bytes1.
+    rewrite <- app_comm_cons in bytes_valid.
+    destruct bytes3. specialize (encoder_spec_injective encoder encoder_spec_compliant [] [code2] [] encode_nil encode_code2) as G. inversion G.
+Admitted.
+    (* destruct_valid_bytes bytes_valid. *)
+
+    
+   
+Theorem decode_encode_spec_compliant_decode_inverse_of_encode : forall encoder decoder,
+    utf8_encoder_spec encoder ->
+    utf8_decoder_spec decoder ->
+    forall (codes_big codes: list codepoint) bytes codes_suffix,
+      (length codes) <= (length codes_big) ->
+      encoder codes = (bytes, codes_suffix) ->
+      exists codes_prefix, decoder bytes = (codes_prefix, nil) /\ codes = (codes_prefix ++ codes_suffix)%list.
+Proof.
+  intros encoder decoder encoder_spec_compliant decoder_spec_compliant.
+  assert (G1 := encoder_spec_compliant).
+  assert (G2 := decoder_spec_compliant).
+  unfold utf8_encoder_spec, encoder_encode_correctly_implies_valid, encoder_encode_valid_codes_correctly, encoder_strictly_increasing in G1.
+  destruct G1 as [enc_implies_valid_utf8_bytes [valid_codepoints_iff_enc [enc_strictly_increasing enc_projects]]].
+  unfold utf8_decoder_spec, decoder_decode_correctly_implies_valid, decoder_decode_valid_utf8_bytes_correctly, decoder_strictly_increasing in G2.
+  destruct G2 as [dec_implies_valid [valid_implies_dec dec_strictly_increasing]].
+  induction codes_big; intros codes bytes codes_suffix less_than encoder_codes.
+  - inversion less_than. apply length_zero_iff_nil in H0. subst.
+    specialize (encoder_spec_implies_nil_mapsto_nil encoder encoder_spec_compliant) as encode_nil.
+    rewrite encode_nil in encoder_codes. inversion encoder_codes. exists [].
+    split. apply decoder_spec_nil_mapsto_nil. apply decoder_spec_compliant. reflexivity.
+  - apply enc_implies_valid_utf8_bytes in encoder_codes as [bytes_valid [codes_prefix [codes_prefix_eq encoder_codes_prefix]]].
+    exists codes_prefix. destruct codes_prefix.
+    + rewrite encoder_spec_implies_nil_mapsto_nil in encoder_codes_prefix. 2: apply encoder_spec_compliant. inversion encoder_codes_prefix. split. apply decoder_spec_nil_mapsto_nil. apply decoder_spec_compliant. assumption.
+    + split; [| apply codes_prefix_eq].
+      replace (c :: codes_prefix) with ([c] ++ codes_prefix) in encoder_codes_prefix by reflexivity.
+      rewrite enc_projects in encoder_codes_prefix.
+      destruct (encoder [c]) as [bytes1 c_rest]  eqn:encoder_c.
+      destruct (encoder codes_prefix) as [bytes2 codes_rest] eqn:encoder_codes_prefix2.
+      destruct c_rest; try discriminate. inversion encoder_codes_prefix. subst.
+      rewrite length_app in less_than.
+      clear encoder_codes_prefix.
+      apply enc_implies_valid_utf8_bytes in encoder_c as G1, encoder_codes_prefix2 as G2.
+      destruct G1 as [bytes1_valid _]. destruct G2 as [bytes2_valid _].
+      simpl in less_than. apply IHcodes_big in encoder_codes_prefix2. 2: lia.
+      rewrite decoder_spec_decode_app_valid_bytes; try assumption.
+      destruct encoder_codes_prefix2 as [codes_prefix2 [decoder_bytes2 codes_prefix2_eq]]. subst.
+      rewrite decoder_bytes2. apply valid_implies_dec in bytes1_valid as [codes decode_bytes1].
+      rewrite decode_bytes1. rewrite app_nil_r.
+      rewrite pair_equal_spec. split; [| reflexivity].
+      replace (c :: codes_prefix2) with ([c] ++ codes_prefix2) by reflexivity.
+      clear decoder_bytes2. clear bytes2_valid.
+      apply app_inv_tail_iff.
 
 Theorem encoder_spec_implies_encode_single_equals : forall encoder1 code bytes,
     utf8_encoder_spec encoder1 ->
@@ -263,70 +384,6 @@ Qed.
 (*   rewrite enc1_strictly_increasing in enc2_strictly_increasing. *)
   
 (* Admitted. *)
-
-Lemma decoder_spec_injective : forall decoder,
-    utf8_decoder_spec decoder ->
-    forall (bytes1 bytes2: list byte) codes,
-      decoder bytes1 = (codes, []) ->
-      decoder bytes2 = (codes, []) ->
-      bytes1 = bytes2.
-Proof.
-  intros decoder decoder_spec_compliant.
-  assert (G := decoder_spec_compliant).
-  unfold utf8_decoder_spec, decoder_decode_correctly_implies_valid, decoder_decode_valid_utf8_bytes_correctly, decoder_strictly_increasing in G.
-  destruct G as [dec_implies_valid_utf8_bytes [valid_bytes_iff_enc dec_strictly_increasing]].
-  intros bytes1 bytes2 codes decoder_bytes1 decoder_bytes2.
-  specialize (dec_strictly_increasing bytes1 bytes2 codes codes decoder_bytes1 decoder_bytes2) as compare_codes.
-  unfold codepoints_compare in compare_codes.
-  rewrite list_compare_refl_if in compare_codes. 2: apply Z.compare_eq_iff.
-  unfold bytes_compare in compare_codes. symmetry in compare_codes. rewrite list_compare_refl in compare_codes.
-  apply compare_codes. apply byte_compare_eq_iff.
-Qed.
-
-Lemma decoder_spec_nil_mapsto_nil : forall decoder,
-    utf8_decoder_spec decoder ->
-    decoder nil = (nil, []).
-  intros decoder decoder_spec_compliant.
-  assert (G := decoder_spec_compliant).
-  unfold utf8_decoder_spec, decoder_decode_correctly_implies_valid, decoder_decode_valid_utf8_bytes_correctly, decoder_strictly_increasing in G.
-  destruct G as [dec_implies_valid_utf8_bytes [valid_bytes_iff_enc dec_strictly_increasing]].
-  assert (valid_utf8_bytes []) as nil_valid. constructor. apply valid_bytes_iff_enc in nil_valid.
-  destruct nil_valid.
-  
-  Admitted.
-
-Theorem decode_encode_spec_compliant_decode_inverse_of_encode : forall encoder decoder,
-    utf8_encoder_spec encoder ->
-    utf8_decoder_spec decoder ->
-    forall codes bytes codes_suffix,
-      encoder codes = (bytes, codes_suffix) ->
-      exists codes_prefix, decoder bytes = (codes_prefix, nil) /\ codes = (codes_prefix ++ codes_suffix)%list.
-Proof.
-  intros encoder decoder encoder_spec_compliant decoder_spec_compliant.
-  assert (G1 := encoder_spec_compliant).
-  assert (G2 := decoder_spec_compliant).
-  unfold utf8_encoder_spec, encoder_encode_correctly_implies_valid, encoder_encode_valid_codes_correctly, encoder_strictly_increasing in G1.
-  destruct G1 as [enc_implies_valid_utf8_bytes [valid_codepoints_iff_enc [enc_strictly_increasing enc_projects]]].
-  unfold utf8_decoder_spec, decoder_decode_correctly_implies_valid, decoder_decode_valid_utf8_bytes_correctly, decoder_strictly_increasing in G2.
-  destruct G2 as [dec_implies_valid [valid_implies_dec dec_strictly_increasing]].
-  intros codes bytes codes_suffix encoder_codes.
-  apply enc_implies_valid_utf8_bytes in encoder_codes as G.
-  destruct G as [bytes_valid [codes_prefix [codes_prefix_eq encoder_prefix]]].
-  exists codes_prefix. split; [| apply codes_prefix_eq]. clear encoder_codes. clear codes_prefix_eq.
-  apply valid_implies_dec in bytes_valid.
-  destruct bytes_valid as [codes2 decode_bytes].
-  apply dec_implies_valid in decode_bytes as G.
-  destruct G as [codes2_valid _].
-  apply valid_codepoints_iff_enc in codes2_valid.
-  destruct codes2_valid as [bytes2 encoder_codes2].
-  specialize (enc_strictly_increasing codes_prefix codes2 bytes bytes2 encoder_prefix encoder_codes2).
-  apply enc_implies_valid_utf8_bytes in encoder_codes2.
-  destruct encoder_codes2 as [bytes2_valid _].
-  apply valid_implies_dec in bytes2_valid as [codes3 decode_bytes2].
-  specialize (dec_strictly_increasing bytes bytes2 codes2 codes3 decode_bytes decode_bytes2).
-  rewrite <- enc_strictly_increasing in dec_strictly_increasing.
-  symmetry in dec_strictly_increasing.
-Qed.
 
 (*   intros encoder decoder encoder_spec_compliant decoder_spec_compliant. *)
 (*   unfold utf8_encoder_spec, encoder_encode_correctly_implies_valid, encoder_encode_valid_codes_correctly, encoder_injective in encoder_spec_compliant. *)
